@prefix dct: <http://purl.org/dc/terms/> .
@prefix ex-voc: <https://github.com/fair-data-collective/excel2rdf-template/> .
@prefix foaf: <http://xmlns.com/foaf/0.1/> .
@prefix owl: <http://www.w3.org/2002/07/owl#> .
@prefix rdf: <http://www.w3.org/1999/02/22-rdf-syntax-ns#> .
@prefix skos: <http://www.w3.org/2004/02/skos/core#> .
@prefix xsd: <http://www.w3.org/2001/XMLSchema#> .

<https://github.com/fair-data-collective/excel2rdf-template> a skos:ConceptScheme;
  dct:contributor <https://orcid.org/0000-0001-8888-635X>;
  dct:created "2022-06-01T00:00:00+00:00"^^xsd:datetime;
  dct:creator <https://orcid.org/0000-0001-6875-5360>, <https://orcid.org/0000-0002-9381-9693>,
    <https://orcid.org/0000-0003-2195-3997>;
  dct:description "This is a template for building a SKOS-based controlled vocabulary. It is used as base of the worflow described in excel2rdf.readthedocs.io/"@en;
  dct:modified "2025-05-29T17:18:00-07:00"^^xsd:datetime;
  dct:rights <https://spdx.org/licenses/CC0-1.0>;
  dct:title "Example template for building SKOS vocabularies"@en;
  owl:versionInfo "0.5.0"@en;
  skos:hasTopConcept ex-voc:VeryTopConcept;
  skos:prefLabel "Example template for building SKOS vocabularies"@en;
  foaf:homepage <https://github.com/fair-data-collective/excel2rdf-template> .

ex-voc:VeryTopConcept a skos:Concept;
  dct:creator <https://orcid.org/0000-0001-6875-5360>;
  skos:altLabel "Root Concept"@en;
  skos:definition "In this vocabulary this Is a root concept for the whole vocabulary"@en;
  skos:inScheme <https://github.com/fair-data-collective/excel2rdf-template>;
  skos:narrower ex-voc:TopConceptOne, ex-voc:TopConceptTwo;
  skos:prefLabel "Very Top Concept"@en;
  skos:topConceptOf <https://github.com/fair-data-collective/excel2rdf-template> .

ex-voc:TopConceptOne a skos:Concept;
  dct:contributor <https://orcid.org/0000-0001-6875-5360>;
  dct:creator <https://orcid.org/0000-0002-9381-9693>;
  skos:altLabel "Best Concept"@en, "First Concept"@en;
  skos:broader ex-voc:VeryTopConcept;
  skos:definition "This is a top concept which is used to collect a number of narrower concepts."@en;
  skos:inScheme <https://github.com/fair-data-collective/excel2rdf-template>;
  skos:narrower ex-voc:NarrowConceptOne, ex-voc:NarrowConceptTwo;
  skos:prefLabel "Top Concept One"@en .

ex-voc:NarrowConceptOne a skos:Concept;
  dct:creator <https://orcid.org/0000-0001-6875-5360>;
  skos:broader ex-voc:TopConceptOne;
  skos:definition "A definition of NarrowConceptOne, which has a broader concept TopConceptOne."@en;
  skos:inScheme <https://github.com/fair-data-collective/excel2rdf-template>;
  skos:prefLabel "Narrow Concept One"@en .

ex-voc:NarrowConceptTwo a skos:Concept;
  dct:creator <https://orcid.org/0000-0001-6875-5360>;
  skos:broader ex-voc:TopConceptOne;
  skos:definition "A definition of NarrowConceptTwo, which has a broader concept TopConceptOne."@en;
  skos:inScheme <https://github.com/fair-data-collective/excel2rdf-template>;
  skos:prefLabel "Narrow Concept Two"@en .

ex-voc:TopConceptTwo a skos:Concept;
  dct:contributor <https://orcid.org/0000-0001-6875-5360>;
  dct:creator <https://orcid.org/0000-0002-9381-9693>;
  skos:altLabel "Last Concept"@en, "Second Concept"@en;
  skos:broader ex-voc:VeryTopConcept;
  skos:definition "This is yet another top concept which is used to collect a number of narrower concepts."@en;
  skos:inScheme <https://github.com/fair-data-collective/excel2rdf-template>;
  skos:prefLabel "Top Concept Two"@en .

ex-voc:NarrowConceptThree a skos:Concept;
  dct:contributor <https://orcid.org/0000-0001-6875-5360>;
  dct:creator <https://orcid.org/0000-0002-9381-9693>;
  skos:broader "temp-vocab:TopConceptTwo"@en;
  skos:definition "A definition of NarrowConceptThree, which has a broader concept TopConceptTwo."@en;
  skos:inScheme <https://github.com/fair-data-collective/excel2rdf-template>;
  skos:prefLabel "Narrow Concept Three"@en .

ex-voc:NarrowConceptFour a skos:Concept;
  dct:contributor <https://orcid.org/0000-0001-6875-5360>;
  dct:creator <https://orcid.org/0000-0002-9381-9693>;
  skos:broader "temp-vocab:TopConceptTwo"@en;
  skos:definition "A definition of NarrowConceptFour, which has a broader concept TopConceptTwo."@en;
  skos:inScheme <https://github.com/fair-data-collective/excel2rdf-template>;
  skos:prefLabel "Narrow Concept Four"@en .
